coq/Primitives.v
@@ -44,16 +44,26 @@ Module PrimUntyped.
   | USubstField (f: string)
   | USubstFieldBits (sig: struct_sig) (f: string).
 
+  Inductive uarray1 :=
+  | UGetElement (pos: nat)
+  | UGetElementBits (sig: array_sig) (pos: nat).
+
+  Inductive uarray2 :=
+  | USubstElement (pos: nat)
+  | USubstElementBits (sig: array_sig) (pos: nat).
+
   Inductive ufn1 :=
   | UDisplay (fn: udisplay)
   | UConv (fn: uconv)
   | UBits1 (fn: ubits1)
-  | UStruct1 (fn: ustruct1).
+  | UStruct1 (fn: ustruct1)
+  | UArray1 (fn: uarray1).
 
   Inductive ufn2 :=
   | UEq
   | UBits2 (fn: ubits2)
-  | UStruct2 (fn: ustruct2).
+  | UStruct2 (fn: ustruct2)
+  | UArray2 (fn: uarray2).
 End PrimUntyped.
 
 Module PrimTyped.
@@ -94,16 +104,30 @@ Module PrimTyped.
   Inductive fstruct2 :=
   | SubstField.
 
+  Inductive farray1 :=
+  | GetElement.
+
+  Inductive farray2 :=
+  | SubstElement.
+
   Inductive fn1 :=
   | Display (fn: fdisplay)
   | Conv (tau: type) (fn: fconv)
   | Bits1 (fn: fbits1)
-  | Struct1 (fn: fstruct1) (sig: struct_sig) (f: struct_index sig).
+  | Struct1 (fn: fstruct1) (sig: struct_sig) (f: struct_index sig)
+  | Array1 (fn: farray1) (sig: array_sig) (idx: array_index sig).
 
   Inductive fn2 :=
   | Eq (tau: type)
   | Bits2 (fn: fbits2)
-  | Struct2 (fn: fstruct2) (sig: struct_sig) (f: struct_index sig).
+  | Struct2 (fn: fstruct2) (sig: struct_sig) (f: struct_index sig)
+  | Array2 (fn: farray2) (sig: array_sig) (idx: array_index sig).
+
+  Definition GetElementBits (sig: array_sig) (idx: array_index sig) : fbits1 :=
+    Slice (array_sz sig) (element_offset_right sig idx) (element_sz sig).
+
+  Definition SubstElementBits (sig: array_sig) (idx: array_index sig) : fbits2 :=
+    SliceSubst (array_sz sig) (element_offset_right sig idx) (element_sz sig).
 
   Definition GetFieldBits (sig: struct_sig) (idx: struct_index sig) : fbits1 :=
     Slice (struct_sz sig) (field_offset_right sig idx) (field_sz sig idx).
@@ -118,13 +142,16 @@ Module PrimTypeInference.
   Definition find_field sig f : result _ fn_tc_error :=
     opt_result (List_assoc f sig.(struct_fields)) (Arg1, UnboundField f sig).
 
+  Definition check_index sig pos : result (array_index sig) fn_tc_error :=
+    opt_result (Vect.index_of_nat sig.(array_len) pos) (Arg1, OutOfBounds pos sig).
+
   Definition tc1 (fn: ufn1) (tau1: type): result fn1 fn_tc_error :=
     match fn with
     | UDisplay fn =>
       match fn with
       | UDisplayUtf8 =>
-        let/res sz1 := assert_bits_t Arg1 tau1 in
-        Success (Display (DisplayUtf8 sz1))
+        let/res sig := assert_kind (kind_array None) Arg1 tau1 in
+        Success (Display (DisplayUtf8 sig.(array_len)))
       | UDisplayValue =>
         Success (Display (DisplayValue tau1))
       end
@@ -135,7 +162,7 @@ Module PrimTypeInference.
                | UIgnore => Conv tau1 Ignore
                end)
     | UBits1 fn =>
-      let/res sz1 := assert_bits_t Arg1 tau1 in
+      let/res sz1 := assert_kind kind_bits Arg1 tau1 in
       Success (Bits1 match fn with
                      | UNot => Not sz1
                      | USExt width => SExt sz1 width
@@ -147,12 +174,22 @@ Module PrimTypeInference.
     | UStruct1 fn =>
       match fn with
       | UGetField f =>
-        let/res sig := assert_struct_t Arg1 tau1 in
+        let/res sig := assert_kind (kind_struct None) Arg1 tau1 in
         let/res idx := find_field sig f in
         Success (Struct1 GetField sig idx)
       | UGetFieldBits sig f =>
         let/res idx := find_field sig f in
         Success (Bits1 (GetFieldBits sig idx))
+      end
+    | UArray1 fn =>
+      match fn with
+      | UGetElement pos =>
+        let/res sig := assert_kind (kind_array None) Arg1 tau1 in
+        let/res idx := check_index sig pos in
+        Success (Array1 GetElement sig idx)
+      | UGetElementBits sig pos =>
+        let/res idx := check_index sig pos in
+        Success (Bits1 (GetElementBits sig idx))
       end
     end.
 
@@ -160,8 +197,8 @@ Module PrimTypeInference.
     match fn with
     | UEq => Success (Eq tau1)
     | UBits2 fn =>
-      let/res sz1 := assert_bits_t Arg1 tau1 in
-      let/res sz2 := assert_bits_t Arg2 tau2 in
+      let/res sz1 := assert_kind kind_bits Arg1 tau1 in
+      let/res sz2 := assert_kind kind_bits Arg2 tau2 in
       Success (Bits2 match fn with
                      | USel => Sel sz1
                      | USliceSubst offset width => SliceSubst sz1 offset width
@@ -180,12 +217,22 @@ Module PrimTypeInference.
     | UStruct2 fn =>
       match fn with
       | USubstField f =>
-        let/res sig := assert_struct_t Arg1 tau1 in
+        let/res sig := assert_kind (kind_struct None) Arg1 tau1 in
         let/res idx := find_field sig f in
         Success (Struct2 SubstField sig idx)
       | USubstFieldBits sig f =>
         let/res idx := find_field sig f in
         Success (Bits2 (SubstFieldBits sig idx))
+      end
+    | UArray2 fn =>
+      match fn with
+      | USubstElement pos =>
+        let/res sig := assert_kind (kind_array None) Arg1 tau1 in
+        let/res idx := check_index sig pos in
+        Success (Array2 SubstElement sig idx)
+      | USubstElementBits sig pos =>
+        let/res idx := check_index sig pos in
+        Success (Bits2 (SubstElementBits sig idx))
       end
     end.
 End PrimTypeInference.
@@ -237,18 +284,20 @@ Module PrimSignatures.
       end
     | Display fn =>
       {$ match fn with
-         | DisplayUtf8 sz => bits_t sz
+         | DisplayUtf8 len => array_t {| array_len := len; array_type := bits_t 8 |}
          | DisplayValue tau => tau
          end ~> unit_t $}
     | Bits1 fn => Sig_of_CSig (CSigma1 fn)
     | Struct1 GetField sig idx => {$ struct_t sig ~> field_type sig idx $}
+    | Array1 GetElement sig idx => {$ array_t sig ~> sig.(array_type) $}
     end.
 
   Definition Sigma2 (fn: fn2) : Sig 2 :=
     match fn with
     | Eq tau => {$ tau ~> tau ~> bits_t 1 $}
-    | Struct2 SubstField sig idx => {$ struct_t sig ~> field_type sig idx ~> struct_t sig $}
     | Bits2 fn => Sig_of_CSig (CSigma2 fn)
+    | Struct2 SubstField sig idx => {$ struct_t sig ~> field_type sig idx ~> struct_t sig $}
+    | Array2 SubstElement sig idx => {$ array_t sig ~> sig.(array_type) ~> array_t sig $}
     end.
 End PrimSignatures.
 
@@ -376,6 +425,7 @@ Module PrimSpecs.
       end
     | Bits1 fn => CircuitPrimSpecs.sigma1 fn
     | Struct1 GetField sig idx => fun s => get_field sig.(struct_fields) s idx
+    | Array1 GetElement sig idx => fun a => vect_nth a idx
     end.
 
   Definition sigma2 (fn: fn2) : Sig_denote (PrimSignatures.Sigma2 fn) :=
@@ -383,5 +433,6 @@ Module PrimSpecs.
     | Eq tau => fun v1 v2 => if eq_dec v1 v2 then Ob~1 else Ob~0
     | Bits2 fn => CircuitPrimSpecs.sigma2 fn
     | Struct2 SubstField sig idx => fun s v => subst_field sig.(struct_fields) s idx v
+    | Array2 SubstElement sig idx => fun a e => vect_replace a idx e
     end.
 End PrimSpecs.
